code/ecdsa/Hacl.Impl.EC.Masking.ScalarAccess.fst
@@ -13,6 +13,10 @@ open Spec.ECC
 open Spec.ECC.Curves
 open Hacl.Impl.EC.Masking
 
+open Hacl.Spec.EC.Definition
+open Hacl.Impl.EC.PointDouble
+
+
 #set-options " --z3rlimit 200"
 
 
@@ -81,3 +85,89 @@ let getScalar_4 #a scalar i =
   result
 
 
+val getPointPrecomputedMixed: #c: curve -> scalar: lbuffer uint8 (size 32) -> 
+  i:size_t{v i < 256} -> pointToAdd: lbuffer uint64 (size 8) ->
+  Stack unit 
+  (requires fun h -> True)
+  (ensures fun h0 _ h1 -> True)
+
+
+open Hacl.Impl.EC.Precomputed
+
+
+let getPointPrecomputedMixed #c scalar i pointToAdd = 
+  let bits: uint32 = getScalar_4 scalar i in 
+
+  let pointToAdd = create (size 8) (u64 0) in 
+
+  let invK h (k: nat) = True in 
+  Lib.Loops.for 0ul 16ul invK
+  (fun k -> 
+      let mask = eq_mask (to_u64 bits) (to_u64 k) in 
+      (* eq_mask_lemma d (to_u64 k);  *)
+	
+      let lut_cmb_x = sub (points_radix_16 #c) (k *! 8) (size 4) in 
+      let lut_cmb_y = sub (points_radix_16 #c) (k *! 8 +! (size 4)) (size 4) in 
+
+      copy_conditional #c (sub pointToAdd (size 0) (size 4)) lut_cmb_x mask;
+      copy_conditional #c (sub pointToAdd (size 4) (size 4)) lut_cmb_y mask
+    )
+
+
+
+[@ CInline]
+inline_for_extraction noextract  
+val montgomery_ladder_step_radix_precomputed: #c: curve ->
+  p: point c -> tempBuffer: lbuffer uint64 (size 88) -> 
+  scalar:  lbuffer uint8 (size 32)-> 
+  i:size_t{v i < 256} -> 
+  Stack unit
+  (requires fun h -> live h p /\live h tempBuffer /\ live h scalar /\
+    LowStar.Monotonic.Buffer.all_disjoint [loc p;loc tempBuffer; loc scalar])
+  (ensures fun h0 _ h1 -> True)
+
+
+let montgomery_ladder_step_radix_precomputed #c p tempBuffer scalar i =  
+  let bits: uint32 = getScalar_4 scalar i in 
+
+  let pointToAdd = create (size 8) (u64 0) in 
+  getPointPrecomputedMixed #c scalar i pointToAdd;
+  
+  point_double p p tempBuffer;
+  point_double p p tempBuffer;
+  point_double p p tempBuffer;
+  point_double p p tempBuffer (*;
+
+  
+  Hacl.Impl.P256.MixedPointAdd.point_add_mixed p pointToAdd p tempBuffer *)
+
+
+
+inline_for_extraction noextract
+val montgomery_ladder_2_precomputed: #c: curve -> #buf_type: buftype -> p: point c -> 
+  scalar: lbuffer_t buf_type uint8 (size 32) -> 
+  tempBuffer:  lbuffer uint64 (size 88)  -> 
+  Stack unit
+  (requires fun h -> True )
+  (ensures fun h0 _ h1 -> modifies (loc p |+| loc tempBuffer) h0 h1)
+
+let montgomery_ladder_2_precomputed #c #a p scalar tempBuffer =  
+ let h0 = ST.get() in 
+  let inv h (i: nat {i <= 64}) = True in 
+
+ 
+  let bits: uint32 = getScalar_4 scalar 0 in 
+  let pointToStart = sub (points_radix_16 #c) (bits *. size 8) (size 8) in 
+
+  copy (sub p (size 0) (size 8)) pointToStart;
+
+  upd p (size 8) (u64 1);
+  upd p (size 9) (u64 0);
+  upd p (size 10) (u64 0);
+  upd p (size 11) (u64 0);
+
+
+  for 1ul 64ul inv 
+    (fun i -> let h2 = ST.get() in
+      montgomery_ladder_step_radix_precomputed p tempBuffer scalar i
+    )
