code/ecdsa/Hacl.Impl.EC.PointAddMixed.fst
@@ -1,0 +1,1020 @@
+module Hacl.Impl.EC.PointAddMixed
+
+open FStar.HyperStack.All
+open FStar.HyperStack
+module ST = FStar.HyperStack.ST
+
+open Lib.IntTypes
+open Hacl.Impl.EC.Arithmetics
+
+open Lib.Buffer
+
+open Hacl.Impl.EC.LowLevel
+open Hacl.Impl.EC.MontgomeryMultiplication
+open Spec.ECC
+
+open FStar.Tactics 
+open FStar.Tactics.Canon
+
+open FStar.Math.Lemmas
+open Hacl.Impl.EC.Masking
+open Hacl.Spec.EC.Definition
+
+
+open Hacl.Spec.MontgomeryMultiplication
+open FStar.Mul
+
+open Hacl.Impl.P.PointAdd.Aux
+
+
+#set-options "--z3rlimit 300 --ifuel 0 --fuel 0"  
+
+inline_for_extraction noextract
+val copy_point_conditional: #c: curve -> x3_out: felem c -> y3_out: felem c -> z3_out: felem c -> p: point c -> mask: point c ->
+  Stack unit
+  (requires fun h -> 
+    live h x3_out /\ live h y3_out /\ live h z3_out /\ live h p /\ live h mask /\ 
+    LowStar.Monotonic.Buffer.all_disjoint [loc x3_out; loc y3_out; loc z3_out; loc p; loc mask])
+  (ensures fun h0 _ h1 -> modifies (loc x3_out |+| loc y3_out |+| loc z3_out) h0 h1 /\ (
+    let mask = point_z_as_nat c h0 mask in 
+    let x, y, z = point_x_as_nat c h0 p, point_y_as_nat c h0 p, point_z_as_nat c h0 p in
+    if mask = 0 then 
+      as_nat c h1 x3_out == x /\
+      as_nat c h1 y3_out == y /\ 
+      as_nat c h1 z3_out == z
+    else 
+      as_nat c h1 x3_out == as_nat c h0 x3_out /\ 
+      as_nat c h1 y3_out == as_nat c h0 y3_out /\ 
+      as_nat c h1 z3_out == as_nat c h0 z3_out))
+
+
+let copy_point_conditional #c x3_out y3_out z3_out p maskPoint = 
+  [@inline_let]
+  let len  = getCoordinateLenU64 c in 
+  
+  let z = sub maskPoint (size 2 *! len) len in 
+  let mask = isZero_uint64_CT #c z in 
+  
+  let p_x = sub p (size 0) len in 
+  let p_y = sub p len len in 
+  let p_z = sub p (size 2 *! len) len in 
+
+  copy_conditional x3_out p_x mask;
+  copy_conditional y3_out p_y mask;
+  copy_conditional z3_out p_z mask
+
+
+
+inline_for_extraction noextract 
+val _move_from_jacobian_coordinates: #c: curve -> u1: felem c -> u2: felem c -> 
+  s1: felem c -> s2: felem c -> p: point c -> q: point c -> 
+  tempBuffer4: lbuffer uint64 (size 4 *! getCoordinateLenU64 c) -> 
+  Stack unit (requires fun h ->  
+    live h u1 /\ live h u2 /\ live h s1 /\ live h s2 /\ live h tempBuffer4 /\ live h p /\ 
+    live h q /\ point_eval c h p /\ point_eval c h q /\
+    LowStar.Monotonic.Buffer.all_disjoint [loc tempBuffer4; loc p; loc q; loc u1; loc u2; loc s1; loc s2])
+  (ensures fun h0 _ h1 ->  
+    modifies (loc u1 |+| loc u2 |+| loc s1 |+| loc s2 |+| loc tempBuffer4) h0 h1 /\
+    u1Invariant #c h0 h1 u1 p q /\
+    u2Invariant #c h0 h1 u2 p q /\ 
+    s1Invariant #c h0 h1 s1 p q /\
+    s2Invariant #c h0 h1 s2 p q)
+
+
+let _move_from_jacobian_coordinates #c u1 u2 s1 s2 p q tempBuffer = 
+  let h0 = ST.get() in 
+  
+  [@inline_let]
+  let len = getCoordinateLenU64 c in 
+    
+  let pX = sub p (size 0) len in 
+  let pY = sub p len len in 
+  let pZ = sub p (size 2 *! len) len in 
+
+  let qX = sub q (size 0) len in 
+  let qY = sub q len len in 
+  let qZ = sub q (size 2 *! len) len in  
+
+  let z2Square = sub tempBuffer (size 0) len in 
+  let z1Square = sub tempBuffer len len in 
+  let z2Cube = sub tempBuffer (size 2 *! len) len in 
+  let z1Cube = sub tempBuffer (size 3 *! len) len in  
+
+  let h0 = ST.get() in 
+
+  montgomery_square_buffer_dh #c qZ z2Square; 
+  montgomery_square_buffer_dh #c pZ z1Square;
+
+  montgomery_multiplication_buffer_dh #c z2Square qZ z2Cube;
+  montgomery_multiplication_buffer_dh #c z1Square pZ z1Cube;
+
+  montgomery_multiplication_buffer_dh #c z2Square pX u1;
+  montgomery_multiplication_buffer_dh #c z1Square qX u2;
+    
+  montgomery_multiplication_buffer_dh #c z2Cube pY s1;
+  montgomery_multiplication_buffer_dh #c z1Cube qY s2;
+
+  let prime = getPrime c in 
+  
+  let fromDomain = fromDomain #c in 
+  let toDomain = toDomain #c in   
+  let as_nat = as_nat c in 
+
+  let pxD = fromDomain (as_nat h0 pX) in 
+  let qxD = fromDomain (as_nat h0 qX) in 
+
+  let pyD = fromDomain (as_nat h0 pY) in 
+  let qyD = fromDomain (as_nat h0 qY) in 
+
+  let pzD = fromDomain (as_nat h0 pZ) in 
+  let qzD = fromDomain (as_nat h0 qZ) in 
+
+
+  calc (==)
+  {
+    toDomain ((qzD * qzD % prime) * pxD % prime);
+    (==) {lemma_mod_mul_distr_l (qzD * qzD) pxD prime}
+    toDomain (qzD * qzD * pxD % prime);
+  };  
+    
+
+  calc (==)
+  {
+    toDomain ((pzD * pzD % prime) * qxD % prime);
+    (==) {lemma_mod_mul_distr_l (pzD * pzD) qxD prime}
+    toDomain (pzD * pzD * qxD % prime);
+  };
+
+
+  calc (==)
+  {
+    toDomain (((qzD * qzD % prime) * qzD % prime) * pyD % prime);
+    (==) {lemma_mod_mul_distr_l (qzD * qzD) qzD prime}
+    toDomain ((qzD * qzD * qzD % prime) * pyD % prime);
+    (==) {lemma_mod_mul_distr_l (qzD * qzD * qzD) pyD prime}
+    toDomain (qzD * qzD * qzD * pyD % prime);
+  };
+
+  calc (==) 
+  {
+    toDomain (((pzD * pzD % prime) * pzD % prime) * qyD % prime);
+    (==) {lemma_mod_mul_distr_l (pzD * pzD) pzD prime}
+    toDomain(((pzD * pzD) * pzD % prime) * qyD % prime);
+    (==) {lemma_mod_mul_distr_l (pzD * pzD * pzD) qyD prime}
+    toDomain(pzD * pzD * pzD * qyD % prime);
+  }
+
+
+inline_for_extraction noextract 
+val move_from_jacobian_coordinates: #c: curve -> p: point c -> q: point c -> 
+  t12: lbuffer uint64 (size 12 *! getCoordinateLenU64 c) -> 
+  Stack unit (requires fun h -> 
+    live h t12 /\ live h p /\ live h q /\
+    LowStar.Monotonic.Buffer.all_disjoint [loc t12; loc p; loc q] /\ 
+    point_eval c h p /\ point_eval c h q)
+  (ensures fun h0 _ h1 -> 
+    let u1, u2, s1, s2, _, _, _, _ = getU1HCube t12 in 
+    modifies (loc t12) h0 h1 /\ (
+    u1Invariant #c h0 h1 u1 p q /\
+    u2Invariant #c h0 h1 u2 p q /\ 
+    s1Invariant #c h0 h1 s1 p q /\
+    s2Invariant #c h0 h1 s2 p q))
+
+
+let move_from_jacobian_coordinates #c p q t12 = 
+  [@inline_let]
+  let len = getCoordinateLenU64 c in   
+  
+  let t4 = sub t12 (size 0) (size 4 *! len) in 
+   
+  let u1 = sub t12 (size 4 *! len) len in 
+  let u2 = sub t12 (size 5 *! len) len in 
+  let s1 = sub t12 (size 6 *! len) len in 
+  let s2 = sub t12 (size 7 *! len) len in 
+
+  _move_from_jacobian_coordinates #c u1 u2 s1 s2 p q t4
+
+
+
+inline_for_extraction noextract 
+val _compute_common_params_point_add: #c: curve -> h: felem c -> r: felem c -> uh: felem c -> 
+  hCube: felem c -> u1: felem c -> u2: felem c -> s1: felem c -> s2: felem c -> 
+  t4: lbuffer uint64 (size 4 *! getCoordinateLenU64 c) -> 
+  Stack unit (requires fun h0 -> 
+    live h0 h /\ live h0 r /\ live h0 uh /\ live h0 hCube /\ live h0 t4 /\ 
+    live h0 u1 /\ live h0 u2 /\ live h0 s1 /\ live h0 s2 /\
+    LowStar.Monotonic.Buffer.all_disjoint [loc u1; loc u2; loc s1; loc s2; loc h; loc r; loc uh; loc hCube; loc t4] /\ 
+    felem_eval c h0 u1 /\ felem_eval c h0 u2 /\ felem_eval c h0 s1 /\ felem_eval c h0 s2)
+  (ensures fun h0 _ h1 -> 
+    modifies (loc h |+| loc r |+| loc uh |+| loc hCube |+| loc t4) h0 h1 /\
+    hInvariant #c h1 h u1 u2 /\
+    rInvariant #c h1 r s1 s2 /\
+    uhInvariant #c h1 uh h u1 /\
+    hCubeInvariant #c h1 hCube h
+  )
+
+
+let _compute_common_params_point_add #c h r uh hCube u1 u2 s1 s2 t4 =  
+  [@inline_let]
+  let len = getCoordinateLenU64 c in
+  let temp = sub t4 (size 0) len in 
+  
+  felem_sub u2 u1 h; 
+  felem_sub s2 s1 r;    
+  montgomery_square_buffer_dh h temp;
+    let h1 = ST.get() in   
+  montgomery_multiplication_buffer_dh temp u1 uh;
+  montgomery_multiplication_buffer_dh temp h hCube;
+
+  let prime = getPrime c in 
+  lemma_mod_mul_distr_l (fromDomain #c (as_nat c h1 h) * fromDomain #c (as_nat c h1 h)) (fromDomain #c (as_nat c h1 u1)) prime;
+  lemma_mod_mul_distr_l (fromDomain #c (as_nat c h1 h) * fromDomain #c (as_nat c h1 h)) (fromDomain #c (as_nat c h1 h)) prime
+
+inline_for_extraction noextract
+val compute_common_params_point_add: #c: curve 
+  -> t12: lbuffer uint64 (size 12 *! getCoordinateLenU64 c) -> 
+  Stack unit 
+  (requires fun h0 -> live h0 t12 /\ (
+    let u1, u2, s1, s2, _, _, _, _ = getU1HCube t12 in  
+    felem_eval c h0 u1 /\ felem_eval c h0 u2 /\ felem_eval c h0 s1 /\ felem_eval c h0 s2))
+  (ensures fun h0 _ h1 -> 
+    let  u1, u2, s1, s2, h, r, uh, hCube = getU1HCube t12 in 
+    modifies (loc t12) h0 h1 /\
+    as_nat c h0 u1 == as_nat c h1 u1 /\
+    as_nat c h0 u2 == as_nat c h1 u2 /\
+    as_nat c h0 s1 == as_nat c h1 s1 /\
+    as_nat c h0 s2 == as_nat c h1 s2 /\
+    
+    hInvariant #c h1 h u1 u2 /\
+    rInvariant #c h1 r s1 s2 /\
+    uhInvariant #c h1 uh h u1 /\
+    hCubeInvariant #c h1 hCube h)
+
+
+let compute_common_params_point_add #c t12 =
+  [@inline_let]
+  let len = getCoordinateLenU64 c in
+  lemma_ICuttable_common #c; 
+
+  let t4 = sub t12 (size 0) (size 4 *! len) in 
+
+  let u1 = sub t12 (size 4 *! len) len in 
+  let u2 = sub t12 (size 5 *! len) len in 
+  let s1 = sub t12 (size 6 *! len) len in 
+  let s2 = sub t12 (size 7 *! len) len in
+
+  let h = sub t12 (size 8 *! len) len in 
+  let r = sub t12 (size 9 *! len) len in 
+  let uh = sub t12 (size 10 *! len) len in
+  let hCube = sub t12 (size 11 *! len) len in 
+
+  _compute_common_params_point_add #c h r uh hCube u1 u2 s1 s2 t4
+
+
+inline_for_extraction noextract
+val _computeX3_point_add: #c : curve -> x3: felem c -> hCube: felem c -> uh: felem c -> 
+  r: felem c -> t3: lbuffer uint64 (size 3 *! getCoordinateLenU64 c) ->  
+  Stack unit 
+  (requires fun h0 -> 
+    live h0 x3 /\ live h0 hCube /\ live h0 uh /\ live h0 r /\ live h0 r /\ live h0 t3 /\
+    disjoint hCube t3 /\  disjoint uh t3 /\  disjoint x3 t3 /\ disjoint r t3 /\ 
+    disjoint x3 r /\ disjoint x3 hCube /\ disjoint x3 uh /\
+    felem_eval c h0 hCube /\ felem_eval c h0 uh /\ felem_eval c h0 r)
+  (ensures fun h0 _ h1 -> 
+    modifies (loc x3 |+| loc t3) h0 h1 /\ x3Invariant #c h0 h1 x3 r hCube uh)
+
+
+let _computeX3_point_add #c x3 hCube uh r t3 = 
+  let h0 = ST.get() in
+  [@inline_let]
+  let len = getCoordinateLenU64 c in 
+  
+  let rSquare = sub t3 (size 0) len in 
+  let rH = sub t3 len len in 
+  let twoUh = sub t3 (size 2 *! len) len in 
+  
+  montgomery_square_buffer_dh r rSquare; 
+  felem_sub rSquare hCube rH;
+  multByTwo uh twoUh;
+  felem_sub rH twoUh x3; 
+
+  let prime = getPrime c in 
+  let r = as_nat c h0 r in 
+
+  let as_nat = as_nat c in 
+  let toDomain = toDomain #c in 
+  let fromDomain = fromDomain #c in 
+  
+  calc (==)
+  {
+    toDomain (((((fromDomain r * fromDomain r  % prime) - fromDomain (as_nat h0 hCube)) % prime) - (2 * fromDomain (as_nat h0 uh) % prime)) % prime);
+    (==) {lemma_mod_add_distr (- fromDomain (as_nat h0 hCube)) (fromDomain r * fromDomain r) prime}
+    toDomain (((fromDomain r * fromDomain r - fromDomain (as_nat h0 hCube)) % prime - (2 * fromDomain (as_nat h0 uh) % prime)) % prime);
+    (==) {lemma_mod_sub_distr ((fromDomain r * fromDomain r - fromDomain (as_nat h0 hCube)) % prime) (2 * fromDomain (as_nat h0 uh)) prime}
+    toDomain (((fromDomain r * fromDomain r - fromDomain (as_nat h0 hCube)) % prime - (2 * fromDomain (as_nat h0 uh))) % prime);
+    (==) {lemma_mod_add_distr (- (2 * fromDomain (as_nat h0 uh))) ((fromDomain r * fromDomain r - fromDomain (as_nat h0 hCube))) prime}
+    toDomain ((fromDomain r * fromDomain r - fromDomain (as_nat h0 hCube) - (2 * fromDomain (as_nat h0 uh))) % prime);
+    (==) {_ by (canon())}
+    toDomain ((fromDomain r * fromDomain r - fromDomain (as_nat h0 hCube) - 2 * fromDomain (as_nat h0 uh)) % prime);
+  }
+
+inline_for_extraction noextract
+val computex3_point_add: #c : curve -> hCube: felem c -> uh: felem c -> 
+  r: felem c -> t5: lbuffer uint64 (size 5 *! getCoordinateLenU64 c) ->  
+  Stack unit 
+  (requires fun h0 -> 
+    live h0 hCube /\ live h0 uh /\ live h0 r /\ live h0 t5 /\
+    disjoint hCube t5 /\ disjoint uh t5 /\ disjoint r t5 /\
+    felem_eval c h0 hCube /\ felem_eval c h0 uh /\ felem_eval c h0 r)
+  (ensures fun h0 _ h1 -> 
+    let x3 = gsub t5 (size 0) (getCoordinateLenU64 c) in 
+    modifies (loc t5) h0 h1 /\ 
+    x3Invariant #c h0 h1 x3 r hCube uh)
+
+
+let computex3_point_add #c hCube uh r t4 = 
+  [@inline_let]
+  let len = getCoordinateLenU64 c in 
+  
+  let x3 = sub t4 (size 0) len in 
+  let tempBuffer3 = sub t4 len (size 3 *! len) in 
+  _computeX3_point_add x3 hCube uh r tempBuffer3
+
+
+inline_for_extraction noextract 
+val _computeY3_point_add: #c: curve -> y3: felem c -> s1: felem c -> 
+  hCube: felem c -> uh: felem c -> x3_out: felem c -> r: felem c -> 
+  t3: lbuffer uint64 (size 3 *! getCoordinateLenU64 c) -> 
+  Stack unit 
+    (requires fun h -> 
+      live h y3 /\ live h s1 /\ live h hCube /\ live h uh /\ live h uh /\ live h x3_out /\ live h r /\ live h t3 /\
+      disjoint uh t3 /\ disjoint x3_out t3 /\  disjoint y3 t3 /\
+      disjoint r t3 /\
+      disjoint s1 t3 /\
+      disjoint hCube t3 /\ 
+
+      disjoint y3 s1 /\ disjoint y3 hCube /\ disjoint y3 uh /\ disjoint y3 x3_out /\ disjoint y3 r /\
+      
+      felem_eval c h s1 /\ felem_eval c h hCube /\ felem_eval c h uh /\ felem_eval c h x3_out /\ 
+      felem_eval c h r)
+    (ensures fun h0 _ h1 ->
+      modifies (loc y3 |+| loc t3) h0 h1 /\ y3Invariant #c h0 h1 y3 s1 hCube uh x3_out r)
+      
+
+let _computeY3_point_add #c y3 s1 hCube uh x3 r t3 = 
+  let h0 = ST.get() in
+
+  [@inline_let]
+  let len = getCoordinateLenU64 c in 
+  
+  let s1hCube = sub t3 (size 0) len in 
+  let u1hx3 = sub t3 len len in 
+  let ru1hx3 = sub t3 (size 2 *! len) len in 
+
+  montgomery_multiplication_buffer_dh s1 hCube s1hCube;
+  felem_sub uh x3 u1hx3; 
+  montgomery_multiplication_buffer_dh u1hx3 r ru1hx3; 
+  felem_sub #c ru1hx3 s1hCube y3;
+
+  let h3 = ST.get() in 
+
+
+  let prime = getPrime c in
+
+  let s1D = fromDomain #c (as_nat c h0 s1) in 
+  let hCubeD = fromDomain #c (as_nat c h0 hCube) in 
+  let uhD = fromDomain #c (as_nat c h0 uh) in 
+  let x3D = fromDomain #c (as_nat c h0 x3) in 
+  let rD = fromDomain #c (as_nat c h0 r) in 
+
+  calc (==)
+  {
+    toDomain #c (((uhD - x3D) % prime * rD % prime  - (s1D * hCubeD % prime)) % getPrime c);
+    (==) {lemma_mod_mul_distr_l (uhD - x3D) rD prime}
+    toDomain #c (((uhD - x3D) * rD % prime  - (s1D * hCubeD % prime)) % getPrime c);
+    (==) {_ by (canon())}
+    toDomain #c (((uhD - x3D) * rD % prime  - s1D * hCubeD % prime) % getPrime c);
+    (==) {lemma_mod_sub_distr ((uhD - x3D) * rD % prime) (s1D * hCubeD) prime}
+    toDomain #c (((uhD - x3D) * rD % prime - s1D * hCubeD) % getPrime c);
+    (==) {lemma_mod_add_distr (-s1D * hCubeD) ((uhD - x3D) * rD) prime}
+    toDomain #c (((uhD - x3D) * rD - s1D * hCubeD) % getPrime c);
+  }
+
+inline_for_extraction noextract
+val computeY3_point_add: #c: curve -> s1: felem c -> hCube: felem c -> uh: felem c -> r: felem c -> 
+  t5: lbuffer uint64 (size 5 *! getCoordinateLenU64 c) -> 
+  Stack unit 
+    (requires fun h -> 
+      let x3_out = gsub t5 (size 0) (getCoordinateLenU64 c) in 
+      live h s1 /\ live h hCube /\ live h uh /\ live h r /\ live h t5 /\
+      
+      disjoint uh t5 /\
+      disjoint r t5 /\
+      disjoint s1 t5 /\
+      disjoint hCube t5 /\ 
+      
+      felem_eval c h s1 /\ 
+      felem_eval c h hCube /\
+      felem_eval c h uh /\ 
+      felem_eval c h x3_out /\ 
+      felem_eval c h r)
+    (ensures fun h0 _ h1 -> 
+      let len = getCoordinateLenU64 c in 
+      let x3_out = gsub t5 (size 0) len in 
+      let y3_out = gsub t5 len len in 
+      modifies (loc t5) h0 h1 /\
+      as_nat c h0 x3_out == as_nat c h1 x3_out /\
+      y3Invariant #c h0 h1 y3_out s1 hCube uh x3_out r)
+
+
+let computeY3_point_add #c s1 hCube uh r tempBuffer5 = 
+  let x3 = sub tempBuffer5 (size 0) (getCoordinateLenU64 c) in 
+  let y3 = sub tempBuffer5 (getCoordinateLenU64 c) (getCoordinateLenU64 c) in 
+  let tempBuffer3 = sub tempBuffer5 (size 2 *! getCoordinateLenU64 c) (size 3 *! getCoordinateLenU64 c) in 
+  _computeY3_point_add #c y3 s1 hCube uh x3 r tempBuffer3
+
+
+
+inline_for_extraction noextract 
+val __computeZ3_point_add: #c: curve -> z3: felem  c ->  z1: felem c -> z2: felem c ->
+  h: felem c -> tempBuffer: felem c -> 
+  Stack unit
+  (requires fun h0 -> 
+    live h0 z3 /\ live h0 z1 /\ live h0 z2 /\ live h0 h /\  live h0 tempBuffer /\
+    disjoint z3 z1 /\ disjoint z1 tempBuffer /\ disjoint tempBuffer h /\
+    disjoint h z3 /\ disjoint z2 tempBuffer /\ disjoint z3 z2 /\
+    felem_eval c h0 z1 /\ felem_eval c h0 z2 /\ felem_eval c h0 h)
+  (ensures fun h0 _ h1 ->
+    modifies (loc z3 |+| loc tempBuffer) h0 h1 /\ 
+    z3Invariant #c h0 h1 z3 z1 z2 h)  
+
+
+let __computeZ3_point_add #c z3 z1 z2 h tempBuffer = 
+  let h0 = ST.get() in 
+  let z1z2 = sub tempBuffer (size 0) (getCoordinateLenU64 c) in
+  montgomery_multiplication_buffer_dh z1 z2 z1z2;
+  montgomery_multiplication_buffer_dh z1z2 h z3;
+
+  calc (==)
+  {
+    toDomain #c ((fromDomain #c (as_nat c h0 z1) * fromDomain #c (as_nat c h0 z2) % getPrime c) * fromDomain #c (as_nat c h0 h) % getPrime c);
+    (==) {lemma_mod_mul_distr_l (fromDomain #c (as_nat c h0 z1) * fromDomain #c (as_nat c h0 z2)) (fromDomain #c (as_nat c h0 h)) (getPrime c)}
+    toDomain #c (fromDomain #c (as_nat c h0 z1) * fromDomain #c (as_nat c h0 z2) * fromDomain #c (as_nat c h0 h) % getPrime c);}
+
+
+inline_for_extraction noextract 
+val computeZ3_point_add: #c: curve -> p: point c -> q: point c ->
+  h: felem c -> t5: lbuffer uint64 (size 5 *! getCoordinateLenU64 c) -> 
+  Stack unit 
+  (requires fun h0 -> 
+    live h0 t5 /\ live h0 p /\ live h0 q /\ live h0 h /\ 
+    disjoint t5 p /\ disjoint t5 h /\ disjoint t5 q /\
+    point_eval c h0 p /\ point_eval c h0 q /\ felem_eval c h0 h)
+  (ensures fun h0 _ h1 ->     
+    modifies (loc t5) h0 h1 /\ (
+    let len = getCoordinateLenU64 c in 
+    let z1 = getZ p in 
+    let z2 = getZ q in 
+    
+    let x3, y3, z3 = getXYZ #c t5 in 
+    
+    as_nat c h0 x3 == as_nat c h1 x3 /\
+    as_nat c h0 y3 == as_nat c h1 y3 /\
+    z3Invariant #c h0 h1 z3 z1 z2 h))
+
+let computeZ3_point_add #c p q h t5 = 
+  [@inline_let]
+  let len = getCoordinateLenU64 c in 
+
+  let z1 = sub p (size 2 *! len) len in 
+  let z2 = sub q (size 2 *! len) len in 
+  let z3 = sub t5 (size 2 *! len) len in 
+  let t1 = sub t5 (size 3 *! len) len in 
+
+  __computeZ3_point_add z3 z1 z2 h t1
+
+inline_for_extraction noextract
+val copy_result_point_add: #c: curve 
+  -> t5: lbuffer uint64 (size 5 *! (getCoordinateLenU64 c)) 
+  -> p: point c -> q: point c -> result: point c ->
+  Stack unit 
+    (requires fun h -> live h t5 /\ live h p /\ live h q /\ live h result /\
+      eq_or_disjoint p result /\
+      disjoint t5 result /\
+      LowStar.Monotonic.Buffer.all_disjoint [loc t5; loc p; loc q]
+    )
+    (ensures fun h0 _ h1 -> 
+      let x3_out, y3_out, z3_out = getXYZ #c t5 in 
+      modifies (loc t5 |+| loc result) h0 h1 /\ (
+      if point_z_as_nat c h0 q = 0 then 
+	point_x_as_nat c h1 result == point_x_as_nat c h0 p /\
+	point_y_as_nat c h1 result == point_y_as_nat c h0 p /\ 
+	point_z_as_nat c h1 result == point_z_as_nat c h0 p
+      else if point_z_as_nat c h0 p = 0 then 
+	point_x_as_nat c h1 result == point_x_as_nat c h0 q /\
+	point_y_as_nat c h1 result == point_y_as_nat c h0 q /\ 
+	point_z_as_nat c h1 result == point_z_as_nat c h0 q
+      else 
+	point_x_as_nat c h1 result == as_nat c h0 x3_out /\ 
+	point_y_as_nat c h1 result == as_nat c h0 y3_out /\ 
+	point_z_as_nat c h1 result == as_nat c h0 z3_out )
+    )
+
+
+let copy_result_point_add #c t5 p q result = 
+  let h0 = ST.get() in 
+  [@inline_let]
+  let len = getCoordinateLenU64 c in 
+
+  let x3_out = sub t5 (size 0) len in 
+  let y3_out = sub t5 len len in 
+  let z3_out = sub t5 (size 2 *! len) len in 
+
+  copy_point_conditional x3_out y3_out z3_out q p;
+  copy_point_conditional x3_out y3_out z3_out p q;
+  concat3 len x3_out len y3_out len z3_out result
+
+inline_for_extraction noextract
+val computeXY: #c: curve -> hCube: felem c -> uh: felem c 
+  -> r: felem c -> t5: lbuffer uint64 (size 5 *! getCoordinateLenU64 c) 
+  -> s1: felem c -> h: felem c ->
+  Stack unit 
+  (requires fun h0 -> 
+    live h0 t5 /\ live h0 hCube /\ live h0 uh /\ live h0 r /\ live h0 s1 /\ live h0 h /\
+    felem_eval c h0 hCube /\ felem_eval c h0 uh /\ felem_eval c h0 r /\ 
+    felem_eval c h0 s1 /\ felem_eval c h0 h /\
+    disjoint uh t5 /\ disjoint t5 hCube /\ disjoint hCube t5 /\ disjoint r t5 /\ disjoint t5 s1)
+  (ensures fun h0 _ h1 -> modifies (loc t5) h0 h1 /\ (
+    let x3_out, y3_out, _ = getXYZ #c t5 in 
+    x3Invariant #c h0 h1 x3_out r hCube uh /\
+    y3Invariant #c h0 h1 y3_out s1 hCube uh x3_out r))
+
+let computeXY #c hCube uh r t5 s1 h = 
+  computex3_point_add #c hCube uh r t5; 
+  computeY3_point_add #c s1 hCube uh r t5
+
+
+inline_for_extraction noextract
+val computeXYZ: #c: curve -> p: point c -> q: point c -> hCube: felem c -> uh: felem c 
+  -> r: felem c -> t5: lbuffer uint64 (size 5 *! getCoordinateLenU64 c) 
+  -> s1: felem c -> h: felem c ->
+  Stack unit 
+    (requires fun h0 ->  
+      live h0 p /\ live h0 q /\ live h0 hCube /\ live h0 uh /\ live h0 r /\ live h0 t5 /\ live h0 s1 /\ live h0 h /\
+
+      felem_eval c h0 hCube /\ felem_eval c h0 uh /\ felem_eval c h0 r /\
+      felem_eval c h0 s1 /\ felem_eval c h0 h /\ 
+      
+      point_eval c h0 q /\  point_eval c h0 p /\
+      
+      disjoint hCube t5 /\ disjoint uh t5 /\ disjoint r t5 /\ 
+      disjoint t5 s1 /\ disjoint t5 h /\ disjoint t5 p /\ disjoint t5 q
+    )
+    (ensures fun h0 _ h1 -> modifies (loc t5) h0 h1 /\
+      (
+	let z1, z2 = getZ p, getZ q in 
+	
+	let x3_out, y3_out, z3_out = getXYZ t5 in
+	
+	x3Invariant #c h0 h1 x3_out r hCube uh /\
+	y3Invariant #c h0 h1 y3_out s1 hCube uh x3_out r /\ 
+	z3Invariant #c h0 h1 z3_out z1 z2 h))
+
+
+let computeXYZ #c p q hCube uh r t5 s1 h = 
+    let h0 = ST.get() in 
+  computeXY #c hCube uh r t5 s1 h;  
+    let h1 = ST.get() in 
+    lemma_point_eval c h0 h1 p; 
+    lemma_point_eval c h0 h1 q;
+    lemma_coord_eval c h0 h1 p;
+    lemma_coord_eval c h0 h1 q;
+
+  computeZ3_point_add #c p q h t5
+
+inline_for_extraction noextract
+val __point_add_if_second_branch_impl: #c: curve -> result: point c 
+  -> p: point c -> q: point c 
+  -> u1: felem c -> u2: felem c -> s1: felem c -> s2: felem c 
+  -> r: felem c -> h: felem c -> uh: felem c -> hCube: felem c 
+  -> t5 : lbuffer uint64 (size 5 *! getCoordinateLenU64 c) -> 
+  Stack unit (requires fun h0 -> 
+    live h0 result /\ live h0 t5 /\ live h0 p /\ live h0 q /\ live h0 u1 /\ live h0 u2 /\ live h0 s1 /\ live h0 s2 /\ live h0 r /\ live h0 h /\ live h0 uh /\ live h0 hCube /\
+    
+    point_eval c h0 p /\ point_eval c h0 q /\ 
+   
+    eq_or_disjoint p result /\ disjoint result t5 /\ disjoint p q /\ 
+    felem_eval c h0 r /\ felem_eval c h0 s1 /\ felem_eval c h0 h /\ 
+
+    disjoint hCube t5 /\ disjoint uh t5 /\ disjoint r t5 /\ 
+    disjoint t5 s1 /\ disjoint t5 h /\ 
+    disjoint t5 p /\ disjoint t5 q /\
+    
+    uhInvariant #c h0 uh h u1 /\
+    hCubeInvariant #c h0 hCube h 
+  )
+  (ensures fun h0 _ h1 -> modifies (loc t5 |+| loc result) h0 h1 /\ (
+    let prime = getPrime c in 
+
+    let x3, y3, z3 = point_x_as_nat c h1 result, point_y_as_nat c h1 result, point_z_as_nat c h1 result in
+    let pX, pY, pZ = point_x_as_nat c h0 p, point_y_as_nat c h0 p, point_z_as_nat c h0 p in 
+    let qX, qY, qZ = point_x_as_nat c h0 q, point_y_as_nat c h0 q, point_z_as_nat c h0 q in 
+
+    let pxD, pyD, pzD = fromDomain #c pX, fromDomain #c pY, fromDomain #c pZ in 
+    let qxD, qyD, qzD = fromDomain #c qX, fromDomain #c qY, fromDomain #c qZ in 
+    let x3D, y3D, z3D = fromDomain #c x3, fromDomain #c y3, fromDomain #c z3 in 
+
+    let rD = fromDomain #c (as_nat c h0 r) in  
+    let hD = fromDomain #c (as_nat c h0 h) in 
+    let s1D = fromDomain #c (as_nat c h0 s1) in 
+    let u1D = fromDomain #c (as_nat c h0 u1) in  
+
+    point_eval c h1 result /\ (
+    if qzD = 0 then 
+      x3D == pxD /\ y3D == pyD /\ z3D == pzD
+    else if pzD = 0 then 
+      x3D == qxD /\  y3D == qyD /\ z3D == qzD
+    else 
+      x3 == toDomain #c ((rD * rD - hD * hD * hD - 2 * hD * hD * u1D) % prime) /\ 
+      y3 == toDomain #c (((hD * hD * u1D - fromDomain #c x3) * rD - s1D * hD * hD * hD) % prime) /\
+      z3 == toDomain #c (pzD * qzD * hD % prime))))
+
+
+
+let __point_add_if_second_branch_impl #c result p q u1 u2 s1 s2 r h uh hCube t5 = 
+    let h0 = ST.get() in
+  computeXYZ #c p q hCube uh r t5 s1 h;
+    let h1 = ST.get() in
+  copy_result_point_add t5 p q result;
+    let h2 = ST.get() in
+    lemma_coord_eval c h0 h1 p;
+    lemma_coord_eval c h0 h1 q;
+    lemma_point_add_if #c p q result t5 u1 u2 s1 s2 r h uh hCube h0 h1 h2
+
+inline_for_extraction noextract
+val _point_add_if_second_branch_impl: #c: curve -> result: point c 
+  -> p: point c -> q: point c 
+  -> x3y3z3u1u2s1s2: lbuffer uint64 (size 8 *! getCoordinateLenU64 c) 
+  -> r: felem c -> h: felem c -> uh: felem c -> hCube: felem c 
+  -> t5 : lbuffer uint64 (size 5 *! getCoordinateLenU64 c) -> 
+  Stack unit (requires fun h0 -> 
+
+    let u1, u2, s1, s2 = getU1S2 x3y3z3u1u2s1s2 in 
+
+    live h0 result /\ live h0 x3y3z3u1u2s1s2 /\ live h0 p /\ live h0 q /\ live h0 t5 /\ live h0 r /\ live h0 h /\ live h0 uh /\ live h0 hCube /\
+    point_eval c h0 p /\ point_eval c h0 q /\ 
+   
+    eq_or_disjoint p result /\ disjoint result t5 /\ disjoint p q /\
+    felem_eval c h0 r /\ felem_eval c h0 s1 /\ felem_eval c h0 h /\ 
+
+    disjoint hCube t5 /\ disjoint uh t5 /\ 
+    disjoint r t5 /\ disjoint t5 x3y3z3u1u2s1s2 /\
+    disjoint t5 h /\  
+    disjoint t5 p /\ disjoint t5 q /\
+    
+    
+    uhInvariant #c h0 uh h u1 /\
+    hCubeInvariant #c h0 hCube h 
+  )
+  (ensures fun h0 _ h1 -> modifies (loc t5 |+| loc result) h0 h1 /\ (
+    let prime = getPrime c in 
+
+    let u1, u2, s1, s2 = getU1S2 x3y3z3u1u2s1s2 in 
+  
+    let x3, y3, z3 = point_x_as_nat c h1 result, point_y_as_nat c h1 result, point_z_as_nat c h1 result in
+    let pX, pY, pZ = point_x_as_nat c h0 p, point_y_as_nat c h0 p, point_z_as_nat c h0 p in 
+    let qX, qY, qZ = point_x_as_nat c h0 q, point_y_as_nat c h0 q, point_z_as_nat c h0 q in 
+
+    let pxD, pyD, pzD = fromDomain #c pX, fromDomain #c pY, fromDomain #c pZ in 
+    let qxD, qyD, qzD = fromDomain #c qX, fromDomain #c qY, fromDomain #c qZ in 
+    let x3D, y3D, z3D = fromDomain #c x3, fromDomain #c y3, fromDomain #c z3 in 
+
+    let rD = fromDomain #c (as_nat c h0 r) in  
+    let hD = fromDomain #c (as_nat c h0 h) in 
+    let s1D = fromDomain #c (as_nat c h0 s1) in 
+    let u1D = fromDomain #c (as_nat c h0 u1) in  
+
+    point_eval c h1 result /\ (
+    if qzD = 0 then 
+      x3D == pxD /\ y3D == pyD /\ z3D == pzD
+    else if pzD = 0 then 
+      x3D == qxD /\  y3D == qyD /\ z3D == qzD
+    else 
+      x3 == toDomain #c ((rD * rD - hD * hD * hD - 2 * hD * hD * u1D) % prime) /\ 
+      y3 == toDomain #c (((hD * hD * u1D - fromDomain #c x3) * rD - s1D * hD * hD * hD) % prime) /\
+      z3 == toDomain #c (pzD * qzD * hD % prime))))
+
+
+let _point_add_if_second_branch_impl #c result p q x3y3z3u1u2s1s2 r h uh hCube t5 = 
+  [@inline_let]
+  let len = getCoordinateLenU64 c in 
+
+  lemma_ICuttable_point_add0 #c; 
+
+  let u1 = sub x3y3z3u1u2s1s2 (size 4 *! len) len in 
+  let u2 = sub x3y3z3u1u2s1s2 (size 5 *! len) len in 
+  let s1 = sub x3y3z3u1u2s1s2 (size 6 *! len) len in 
+  let s2 = sub x3y3z3u1u2s1s2 (size 7 *! len) len in 
+  
+  __point_add_if_second_branch_impl result p q u1 u2 s1 s2 r h uh hCube t5 
+
+inline_for_extraction noextract
+val _point_add_if_second_branch_impl0: #c: curve -> result: point c 
+  -> p: point c -> q: point c 
+  -> x3y3z3u1u2s1s2: lbuffer uint64 (size 8 *! getCoordinateLenU64 c) 
+  -> rhuhhCube: lbuffer uint64 (size 4 *! getCoordinateLenU64 c)
+  -> t5 : lbuffer uint64 (size 5 *! getCoordinateLenU64 c) -> 
+  Stack unit (requires fun h0 -> 
+    let u1, u2, s1, s2 = getU1S2 x3y3z3u1u2s1s2 in 
+    let h, r, uh, hCube = getHHCube rhuhhCube in 
+
+    live h0 result /\ live h0 p /\ live h0 q /\ live h0 x3y3z3u1u2s1s2 /\ live h0 rhuhhCube /\ live h0 t5 /\ 
+
+    point_eval c h0 p /\ point_eval c h0 q /\ 
+   
+    eq_or_disjoint p result /\ disjoint result t5 /\ disjoint p q /\
+
+    disjoint hCube t5 /\ disjoint uh t5 /\ 
+    disjoint r t5 /\ disjoint t5 x3y3z3u1u2s1s2 /\
+    disjoint t5 h /\ disjoint t5 p /\ disjoint t5 q /\
+    
+    felem_eval c h0 r /\ felem_eval c h0 s1 /\ felem_eval c h0 h /\ 
+    
+    uhInvariant #c h0 uh h u1 /\
+    hCubeInvariant #c h0 hCube h 
+  )
+  (ensures fun h0 _ h1 -> modifies (loc t5 |+| loc result) h0 h1 /\ (
+    let prime = getPrime c in 
+
+    let u1, u2, s1, s2 = getU1S2 x3y3z3u1u2s1s2 in 
+    let h, r, uh, hCube = getHHCube rhuhhCube in 
+  
+    let x3, y3, z3 = point_x_as_nat c h1 result, point_y_as_nat c h1 result, point_z_as_nat c h1 result in
+    let pX, pY, pZ = point_x_as_nat c h0 p, point_y_as_nat c h0 p, point_z_as_nat c h0 p in 
+    let qX, qY, qZ = point_x_as_nat c h0 q, point_y_as_nat c h0 q, point_z_as_nat c h0 q in 
+
+    let pxD, pyD, pzD = fromDomain #c pX, fromDomain #c pY, fromDomain #c pZ in 
+    let qxD, qyD, qzD = fromDomain #c qX, fromDomain #c qY, fromDomain #c qZ in 
+    let x3D, y3D, z3D = fromDomain #c x3, fromDomain #c y3, fromDomain #c z3 in 
+
+    let rD = fromDomain #c (as_nat c h0 r) in  
+    let hD = fromDomain #c (as_nat c h0 h) in 
+    let s1D = fromDomain #c (as_nat c h0 s1) in 
+    let u1D = fromDomain #c (as_nat c h0 u1) in  
+
+    point_eval c h1 result /\ (
+    if qzD = 0 then 
+      x3D == pxD /\ y3D == pyD /\ z3D == pzD
+    else if pzD = 0 then 
+      x3D == qxD /\  y3D == qyD /\ z3D == qzD
+    else 
+      x3 == toDomain #c ((rD * rD - hD * hD * hD - 2 * hD * hD * u1D) % prime) /\ 
+      y3 == toDomain #c (((hD * hD * u1D - fromDomain  #c x3) * rD - s1D * hD * hD * hD) % prime) /\
+      z3 == toDomain #c (pzD * qzD * hD % prime))))
+
+
+let _point_add_if_second_branch_impl0 #c result p q x3y3z3u1u2s1s2 rhuhhCube tempBuffer5 = 
+  [@inline_let]
+  let len = getCoordinateLenU64 c in 
+
+  let h = sub rhuhhCube (size 0) len in 
+  let r = sub rhuhhCube len len in 
+  let uh = sub rhuhhCube (size 2 *! len) len in 
+  let hCube = sub rhuhhCube (size 3 *! len) len in 
+  
+  _point_add_if_second_branch_impl result p q x3y3z3u1u2s1s2 r h uh hCube tempBuffer5
+
+inline_for_extraction noextract
+val _point_add_if_second_branch_impl1: #c: curve -> result: point c 
+  -> p: point c -> q: point c 
+  -> x3hCube: lbuffer uint64 (size 12 *! getCoordinateLenU64 c) 
+  -> t5 : lbuffer uint64 (size 5 *! getCoordinateLenU64 c) -> 
+  Stack unit (requires fun h0 -> 
+    let  u1, u2, s1, s2, h, r, uh, hCube = getU1HCube x3hCube in 
+
+    live h0 result /\ live h0 p /\ live h0 q /\ live h0 x3hCube /\ live h0 t5 /\ 
+
+    point_eval c h0 p /\ point_eval c h0 q /\ 
+   
+    eq_or_disjoint p result /\ disjoint result t5 /\ disjoint p q /\
+    
+    disjoint t5 x3hCube /\  disjoint t5 p /\ disjoint t5 q /\
+    felem_eval c h0 r /\ felem_eval c h0 s1 /\ felem_eval c h0 h /\ 
+    
+    uhInvariant #c h0 uh h u1 /\
+    hCubeInvariant #c h0 hCube h 
+  )
+  (ensures fun h0 _ h1 -> modifies (loc t5 |+| loc result) h0 h1 /\ (
+    let prime = getPrime c in 
+
+    let  u1, u2, s1, s2, h, r, uh, hCube = getU1HCube x3hCube in 
+  
+    let x3, y3, z3 = point_x_as_nat c h1 result, point_y_as_nat c h1 result, point_z_as_nat c h1 result in
+    let pX, pY, pZ = point_x_as_nat c h0 p, point_y_as_nat c h0 p, point_z_as_nat c h0 p in 
+    let qX, qY, qZ = point_x_as_nat c h0 q, point_y_as_nat c h0 q, point_z_as_nat c h0 q in 
+
+    let pxD, pyD, pzD = fromDomain #c pX, fromDomain #c pY, fromDomain #c pZ in 
+    let qxD, qyD, qzD = fromDomain #c qX, fromDomain #c qY, fromDomain #c qZ in 
+    let x3D, y3D, z3D = fromDomain #c x3, fromDomain #c y3, fromDomain #c z3 in 
+
+    let rD = fromDomain #c (as_nat c h0 r) in  
+    let hD = fromDomain #c (as_nat c h0 h) in 
+    let s1D = fromDomain #c (as_nat c h0 s1) in 
+    let u1D = fromDomain #c (as_nat c h0 u1) in  
+
+    point_eval c h1 result /\ (
+    if qzD = 0 then 
+      x3D == pxD /\ y3D == pyD /\ z3D == pzD
+    else if pzD = 0 then 
+      x3D == qxD /\  y3D == qyD /\ z3D == qzD
+    else 
+      x3 == toDomain #c ((rD * rD - hD * hD * hD - 2 * hD * hD * u1D) % prime) /\ 
+      y3 == toDomain #c (((hD * hD * u1D - fromDomain  #c x3) * rD - s1D * hD * hD * hD) % prime) /\
+      z3 == toDomain #c (pzD * qzD * hD % prime))))
+
+
+
+let _point_add_if_second_branch_impl1 #c result p q x3hCube t5 = 
+  [@inline_let]
+  let len = getCoordinateLenU64 c in 
+  
+  let x3y3z3u1u2s1s2 = sub x3hCube (size 0) (size 8 *! len) in 
+  let rhuhhCube = sub x3hCube (size 8 *! len) (size 4 *! len) in 
+  let h0 = ST.get() in 
+
+  l0 #c x3hCube h0 p q;
+  lemma_disjoint_invariant #c x3hCube t5;
+  _point_add_if_second_branch_impl0 #c result p q x3y3z3u1u2s1s2 rhuhhCube t5
+
+inline_for_extraction noextract
+val _point_add_0: #c: curve -> p: point c -> q: point c -> t12: lbuffer uint64 (size 12 *! getCoordinateLenU64 c) -> 
+  Stack unit 
+    (requires fun h0 ->   
+      live h0 p /\ live h0 q /\ live h0 t12 /\
+      LowStar.Monotonic.Buffer.all_disjoint [loc t12; loc p; loc q] /\ 
+      point_eval c h0 p /\ point_eval c h0 q)
+    (ensures fun h0 _ h1 -> 
+      modifies (loc t12) h0 h1 /\ point_eval c h1 p /\ point_eval c h1 q /\  (
+      let  u1, u2, s1, s2, h, r, uh, hCube = getU1HCube t12 in 
+      
+      u1Invariant #c h0 h1 u1 p q /\
+      u2Invariant #c h0 h1 u2 p q /\ 
+      s1Invariant #c h0 h1 s1 p q /\
+      s2Invariant #c h0 h1 s2 p q /\ 
+      hInvariant #c h1 h u1 u2 /\
+      rInvariant #c h1 r s1 s2 /\
+      uhInvariant #c h1 uh h u1 /\
+      hCubeInvariant #c h1 hCube h))
+      
+  
+let _point_add_0 #c p q t12 = 
+  [@inline_let]
+  let len = getCoordinateLenU64 c in 
+  let h0 = ST.get() in 
+  
+  move_from_jacobian_coordinates p q t12;
+  compute_common_params_point_add t12;
+  let h1 = ST.get() in
+  lemma_point_eval c h0 h1 p;
+  lemma_point_eval c h0 h1 q 
+  
+inline_for_extraction noextract
+val point_add_: #c: curve -> p: point c -> q: point c -> result: point c 
+  -> tempBuffer: lbuffer uint64 (size 17 *! getCoordinateLenU64 c) -> 
+  Stack unit (requires fun h -> 
+    live h p /\ live h q /\ live h result /\ live h tempBuffer /\ 
+    eq_or_disjoint q result /\ disjoint p q /\ disjoint p tempBuffer /\ 
+    disjoint q tempBuffer /\ disjoint p result /\ disjoint result tempBuffer /\  
+    point_eval c h p /\ point_eval c h q)
+  (ensures fun h0 _ h1 -> modifies (loc tempBuffer |+| loc result) h0 h1 /\ point_eval c h1 result /\
+    fromDomainPoint #c #DH (point_as_nat c h1 result) == _point_add #c (fromDomainPoint #c #DH (point_as_nat c h0 p)) (fromDomainPoint #c #DH (point_as_nat c h0 q)))
+
+
+let point_add_ #c p q result tempBuffer = 
+  let h0 = ST.get() in 
+  let t12 = sub tempBuffer (size 0) (size 12 *! getCoordinateLenU64 c) in 
+  let t5 = sub tempBuffer (size 12 *! getCoordinateLenU64 c) (size 5 *! getCoordinateLenU64 c) in 
+
+  _point_add_0 #c p q t12;
+  let h1 = ST.get() in 
+  _point_add_if_second_branch_impl1 result p q t12 t5;
+  
+  let h2 = ST.get() in 
+  lemma_coord_eval c h0 h1 p;
+  lemma_coord_eval c h0 h1 q;
+
+  
+  let prime = getPrime c in 
+
+  let x3, y3, z3 = point_x_as_nat c h2 result, point_y_as_nat c h2 result, point_z_as_nat c h2 result in
+  let pX, pY, pZ = point_x_as_nat c h0 p, point_y_as_nat c h0 p, point_z_as_nat c h0 p in 
+  let qX, qY, qZ = point_x_as_nat c h0 q, point_y_as_nat c h0 q, point_z_as_nat c h0 q in 
+
+  let pxD, pyD, pzD = fromDomain #c pX, fromDomain #c pY, fromDomain #c pZ in 
+  let qxD, qyD, qzD = fromDomain #c qX, fromDomain #c qY, fromDomain #c qZ in 
+  let x3D, y3D, z3D = fromDomain #c x3, fromDomain #c y3, fromDomain #c z3 in 
+
+
+  calc (==)
+  {
+    qzD * qzD * pxD % prime;
+    (==) {_ by (canon())}
+    pxD * (qzD * qzD) % prime; };
+    
+  calc (==)
+  {
+    pzD * pzD * qxD % prime;
+    (==) {_ by (canon())}
+    qxD * (pzD * pzD) % prime;
+  };
+    
+  calc (==)
+  {
+    qzD * qzD * qzD * pyD % prime;
+    (==) {_ by (canon())}
+    pyD * qzD * (qzD * qzD) % prime;
+  };
+
+  calc(==)
+  {
+    pzD * pzD * pzD * qyD % prime;
+    (==) {_ by (canon())}
+    qyD * pzD * (pzD * pzD) % prime;
+  };
+
+
+  let u1D = pxD * (qzD * qzD) % prime in
+  let u2D = qxD * (pzD * pzD) % prime in    
+
+  let s1D = pyD * qzD * (qzD * qzD) % prime in 
+  let s2D = qyD * pzD * (pzD * pzD) % prime in 
+    
+  let hD = (u2D - u1D) % prime in
+  let rD = (s2D - s1D) % prime in  
+
+  calc (==)
+  {
+    (rD * rD - hD * hD * hD - 2 * hD * hD * u1D) % prime;
+    (==) {_ by (canon())}
+    ((rD * rD) - (hD * hD * hD) - (2 * u1D * (hD * hD))) % prime;
+  };
+
+  calc (==)
+  {
+    (((hD * hD * u1D - fromDomain  #c x3) * rD - s1D * hD * hD * hD) % prime);
+    (==) {_ by (canon())}
+    (rD * (u1D * (hD * hD) - fromDomain  #c x3) - s1D * (hD * hD * hD)) % prime;
+  };
+
+  calc (==)
+  {
+    (pzD * qzD * hD % prime);
+    (==) {_ by (canon())}
+    (hD * pzD * qzD) % prime;
+  }
+
+[@CInline]
+val point_add_p256: p: point P256 -> q: point P256 -> result: point P256
+  -> tempBuffer: lbuffer uint64 (size 17 *! getCoordinateLenU64 P256) -> 
+  Stack unit (requires fun h -> 
+    live h p /\ live h q /\ live h result /\ live h tempBuffer /\ 
+    eq_or_disjoint q result /\ disjoint p q /\ disjoint p tempBuffer /\ 
+    disjoint q tempBuffer /\ disjoint p result /\ disjoint result tempBuffer /\  
+    point_eval P256 h p /\ point_eval P256 h q)
+  (ensures fun h0 _ h1 -> modifies (loc tempBuffer |+| loc result) h0 h1 /\ point_eval P256 h1 result /\
+    fromDomainPoint #P256 #DH (point_as_nat P256 h1 result) == _point_add #P256 (fromDomainPoint #P256 #DH (point_as_nat P256 h0 p)) (fromDomainPoint #P256 #DH (point_as_nat P256 h0 q)))
+
+let point_add_p256 p q result tempBuffer = point_add_ #P256 p q result tempBuffer
+
+[@CInline]
+val point_add_p384: p: point P384 -> q: point P384 -> result: point P384
+  -> tempBuffer: lbuffer uint64 (size 17 *! getCoordinateLenU64 P384) -> 
+  Stack unit (requires fun h -> 
+    live h p /\ live h q /\ live h result /\ live h tempBuffer /\ 
+    eq_or_disjoint q result /\ disjoint p q /\ disjoint p tempBuffer /\ 
+    disjoint q tempBuffer /\ disjoint p result /\ disjoint result tempBuffer /\  
+    point_eval P384 h p /\ point_eval P384 h q)
+  (ensures fun h0 _ h1 -> modifies (loc tempBuffer |+| loc result) h0 h1 /\ point_eval P384 h1 result /\
+    fromDomainPoint #P384 #DH (point_as_nat P384 h1 result) == _point_add #P384 (fromDomainPoint #P384 #DH (point_as_nat P384 h0 p)) (fromDomainPoint #P384 #DH (point_as_nat P384 h0 q)))
+
+let point_add_p384 p q result tempBuffer = point_add_ #P384 p q result tempBuffer
+
+[@CInline]
+val point_add_generic: p: point Default -> q: point Default -> result: point Default
+  -> tempBuffer: lbuffer uint64 (size 17 *! getCoordinateLenU64 Default) -> 
+  Stack unit (requires fun h -> 
+    live h p /\ live h q /\ live h result /\ live h tempBuffer /\ 
+    eq_or_disjoint q result /\ disjoint p q /\ disjoint p tempBuffer /\ 
+    disjoint q tempBuffer /\ disjoint p result /\ disjoint result tempBuffer /\  
+    point_eval Default h p /\ point_eval Default h q)
+  (ensures fun h0 _ h1 -> modifies (loc tempBuffer |+| loc result) h0 h1 /\ point_eval Default h1 result /\
+    fromDomainPoint #Default #DH (point_as_nat Default h1 result) == _point_add #Default (fromDomainPoint #Default #DH (point_as_nat Default h0 p)) (fromDomainPoint #Default #DH (point_as_nat Default h0 q)))
+
+let point_add_generic p q result tempBuffer = point_add_ #Default p q result tempBuffer
+
+
+let point_add #c p q result tempBuffer = 
+  match c with 
+  |P256 -> point_add_p256 p q result tempBuffer
+  |P384 -> point_add_p384 p q result tempBuffer
+  |Default -> point_add_generic p q result tempBuffer
