code/ecdsa/Hacl.Impl.EC.PointAddMixed.fsti
@@ -1,0 +1,31 @@
+module Hacl.Impl.EC.PointAddMixed
+
+open FStar.HyperStack.All
+open FStar.HyperStack
+module ST = FStar.HyperStack.ST
+
+open Lib.IntTypes
+open Lib.Buffer
+
+open Hacl.Spec.EC.Definition
+open Spec.ECC
+open Spec.ECC.Curves
+open Hacl.Spec.MontgomeryMultiplication
+
+#set-options "--z3rlimit 100"
+
+let fromDomain #c = fromDomain_ #c #DH
+
+
+inline_for_extraction noextract
+val point_add_mixed: #c: curve -> p: point c -> q: pointAffine c -> result: point c 
+  -> tempBuffer: lbuffer uint64 (size 17 *! getCoordinateLenU64 c) -> 
+  Stack unit (requires fun h -> 
+    live h p /\ live h q /\ live h result /\ live h tempBuffer /\ 
+    eq_or_disjoint q result /\ disjoint p q /\ disjoint p tempBuffer /\ 
+    disjoint q tempBuffer /\ disjoint p result /\ disjoint result tempBuffer /\  
+    point_eval c h p /\ 
+      (let x, y = getXAff q, getYAff q in 
+      felem_eval c h x /\ felem_eval c h y))
+  (ensures fun h0 _ h1 -> modifies (loc tempBuffer |+| loc result) h0 h1 /\ point_eval c h1 result /\
+    fromDomainPoint #c #DH (point_as_nat c h1 result) == _point_add_mixed #c (fromDomainPoint #c #DH (point_as_nat c h0 p)) (fromDomainPointAffine #c (point_affine_as_nat c h0 q)))
